Set_Graphs/Graph_Algorithms/CSR_Graph.thy
@@ -1,0 +1,870 @@
+theory CSR_Graph
+  imports Separation_Logic_Imperative_HOL_Partial.Imp_Map_Spec
+    Directed_Set_Graphs.Pair_Graph_Imperative BFS_Refinement
+begin                       
+
+term nths
+
+value "nths [(0::nat),1,2,3,4,5,6,7,8] (Set.insert 6 {(1::nat)..4})"
+
+lemma intervall_rw1:"{0..ed} = {..< Suc ed}"
+  by auto
+
+lemma intervall_rw2:"{j. j \<le> n} = {..<Suc n}"
+  by auto
+
+lemma nths_intervall_as_drop_and_take:
+  "nths list {start..ed} = drop (start) (take (Suc ed) list)"
+  apply(induction list arbitrary: start ed)
+  subgoal
+    by simp
+  subgoal for a list start ed
+    apply(cases start)
+     apply(all \<open>cases ed\<close>)
+       apply (auto simp add: nths_Cons)
+    subgoal
+      by(auto simp add: intervall_rw2)
+    by(auto simp add: nths_def)
+  done
+
+lemma nths_intervall_split_off_first:
+  assumes "start \<le> end" "end < length list"
+  shows "(nths list {start..end}) =  (list ! start # nths list {Suc start..end})"
+  unfolding nths_intervall_as_drop_and_take
+  apply(subst Cons_nth_drop_Suc[of start, symmetric])
+  using assms(1,2)
+  by (auto intro!: arg_cong2[where f = Cons] simp add: assms(1) le_imp_less_Suc)
+
+lemma nth_shifted_by_lower_bound_of_nths_intervall:
+  assumes "u < length xs" "i \<ge> l" "i \<le> u"
+  shows "nths xs {l..u} ! (i -l) = xs ! i" 
+  unfolding nths_intervall_as_drop_and_take
+  using assms
+  by (subst nth_drop)(auto simp add: le_imp_less_Suc)
+
+lemma nth_of_nths_intervall_shifted_by_lower_bound:
+  assumes "u < length xs" "l + i \<le> u" 
+  shows "nths xs {l..u} ! (i) = xs ! (i + l)" 
+  unfolding nths_intervall_as_drop_and_take
+  using assms
+  by (subst nth_drop)(auto simp add: le_imp_less_Suc algebra_simps)
+
+lemma zip_foldl_map:
+     "ys = map y xs \<Longrightarrow> foldl (\<lambda>acc a. case a of (x, y) \<Rightarrow> f x y acc) acc (zip xs ys)
+      = foldl (\<lambda>acc x. f x (y x) acc) acc xs"
+  by(induction xs arbitrary: acc ys) auto
+
+lemma length_nths_of_intervall:
+  assumes  "u < length xs"
+  shows "length (nths xs {l..u})  = (u + 1) - l" 
+  using assms
+  by(auto simp add: nths_intervall_as_drop_and_take)
+
+partial_function (heap) iterate_range where
+  "iterate_range arr start end fi acc=
+    (if start \<le> end then
+      do{ current \<leftarrow> Array.nth arr start;
+          acc' \<leftarrow> fi current acc;
+          iterate_range arr (Suc start) end fi acc'}
+     else return acc)"
+
+definition "put arr new = Array.upd arr 0 new"
+
+
+lemma iterate_range_rule:
+  assumes "\<And> acc acci x. <acc_assn acc acci * F> fi x acci 
+            <\<lambda> r. acc_assn (f acc x) r * F>"
+  shows "<arr \<mapsto>\<^sub>a list * \<up> (start \<le> length list \<and> end < length list) *F * acc_assn acc acci>
+          iterate_range arr start end fi acci 
+         <\<lambda> r. arr \<mapsto>\<^sub>a list * acc_assn (foldl f acc (nths list {start..end})) r *  F>"
+proof(induction arbitrary: start acc acci rule: iterate_range.fixp_induct, goal_cases)
+  case 1
+  then show ?case
+    by simp
+next
+  case 2
+  then show ?case 
+    by simp
+next
+  case (3 fi start acc acci)
+  note IH = this
+  show ?case 
+     using assms(1) IH(1)[of "Suc start" "f acc _"]
+     by (sep_auto simp: nths_intervall_split_off_first[of start] split: if_split)
+ qed
+
+partial_function (heap) iterate_range_infoed where
+  "iterate_range_infoed arr info_arr start end fi acc=
+    (if start \<le> end then
+      do{ current \<leftarrow> Array.nth arr start;
+          current_info \<leftarrow> Array.nth info_arr start;
+          acc' \<leftarrow> fi current current_info acc;
+          iterate_range_infoed arr info_arr (Suc start) end fi acc'}
+     else return acc)"
+
+lemma iterate_range_infoed_rule:
+  assumes "\<And> acc acci x y. <acc_assn acc acci * F> fi x y acci 
+            <\<lambda> r. acc_assn (f acc (x, y)) r * F>"
+  shows "<arr \<mapsto>\<^sub>a list * info_arr \<mapsto>\<^sub>a info_list *
+          \<up> (start \<le> length list \<and> end < length list \<and>
+             start \<le> length info_list \<and> end < length info_list) *F * acc_assn acc acci>
+          iterate_range_infoed arr info_arr start end fi acci 
+       <\<lambda> r. arr \<mapsto>\<^sub>a list *  info_arr \<mapsto>\<^sub>a info_list * 
+        acc_assn (foldl f acc (zip (nths list {start..end}) (nths info_list {start..end}))) r * F>"
+proof(induction arbitrary: start acc acci rule: iterate_range_infoed.fixp_induct, goal_cases)
+  case 1
+  then show ?case
+    by simp
+next
+  case 2
+  then show ?case 
+    by simp
+next
+  case (3 fi start acc acci)
+  note IH = this
+  show ?case 
+     using assms(1) IH(1)[of "Suc start" "f acc _"]
+     by (sep_auto simp: nths_intervall_split_off_first[of start] split: if_split)
+ qed
+
+locale CSR_map = 
+ imp_map_lookup is_index_map index_lookup
+ for is_index_map and index_lookup::" nat \<Rightarrow> 'indices \<Rightarrow> nat option Heap"
+begin
+
+definition "CSR_assn_raw nhlists Gi sindicesi eindicesi nha sindices eindices= 
+  (Gi \<mapsto>\<^sub>a nha * is_index_map sindices sindicesi
+      * is_index_map eindices eindicesi * 
+       \<up> (dom eindices = dom sindices \<and> dom nhlists = dom sindices \<and>
+          (\<forall> v \<in> dom sindices. (the (sindices v) < length nha  \<and> the (eindices v) < length nha) 
+               \<and> the (nhlists v) = nths nha {the (sindices v)..the (eindices v)})
+         \<and> (\<forall> u v. ({u, v} \<subseteq> dom sindices \<and> u \<noteq> v)
+             \<longrightarrow> {the (sindices v)..the (eindices v)} \<inter> {the (sindices u)..the (eindices v)} = {}))
+       )"
+
+definition "CSR_assn nhlists Gi sindicesi eindicesi = 
+  (\<exists>\<^sub>A nha sindices eindices. CSR_assn_raw nhlists Gi sindicesi eindicesi nha sindices eindices)"
+
+
+definition "iterate_neighbourhood Gi sindicesi eindicesi v fi acci= 
+   do{ vstarto \<leftarrow> index_lookup v sindicesi;
+       case vstarto of None \<Rightarrow> return acci
+       | Some vstart \<Rightarrow> do{
+          vendo \<leftarrow> index_lookup v eindicesi;
+          let vend = the vendo;
+          iterate_range Gi vstart vend (fi v) acci}}"
+
+lemma iterate_neighbourhood_raw_rule:
+  assumes "\<And> acc acci x. <acc_assn acc acci * F> fi v x acci 
+            <\<lambda> r. acc_assn (f v acc x) r * F>"
+  shows "<CSR_assn_raw nhlists Gi sindicesi eindicesi nha sindices eindices* acc_assn acc acci * F>
+         iterate_neighbourhood Gi sindicesi eindicesi v fi acci
+        <\<lambda> r. CSR_assn_raw nhlists Gi sindicesi eindicesi nha sindices eindices* F* 
+              acc_assn (case nhlists v of None \<Rightarrow> acc
+                        | Some vs \<Rightarrow> foldl (f v) acc vs) r>"
+proof-
+  let ?big_assn = "Gi \<mapsto>\<^sub>a nha * is_index_map sindices sindicesi * is_index_map eindices eindicesi *
+     \<up> (dom eindices = dom sindices \<and>
+        dom nhlists = dom sindices \<and>
+        (\<forall>v\<in>dom sindices.
+            (the (sindices v) < length nha \<and> the (eindices v) < length nha) \<and>
+            the (nhlists v) = nths nha {the (sindices v)..the (eindices v)}) \<and>
+        (\<forall>u v. {u, v} \<subseteq> dom sindices \<and> u \<noteq> v \<longrightarrow>
+               {the (sindices v)..the (eindices v)} \<inter> {the (sindices u)..the (eindices v)} = {})) *
+     acc_assn acc acci *F"
+  let ?help_assn ="\<lambda> vstart vend. is_index_map sindices sindicesi * is_index_map eindices eindicesi *
+     \<up> (dom eindices = dom sindices \<and>
+        dom nhlists = dom sindices \<and>
+        (\<forall>v\<in>dom sindices.
+            the (sindices v) < length nha \<and>
+            the (eindices v) < length nha \<and>
+            the (nhlists v) = nths nha {the (sindices v)..the (eindices v)}) \<and>
+        (\<forall>u v. {u, v} \<subseteq> dom sindices \<and> u \<noteq> v \<longrightarrow>
+               {the (sindices v)..the (eindices v)} \<inter> {the (sindices u)..the (eindices v)} = {})) *
+     \<up> (Some vstart = sindices v) *
+     \<up> (Some vend = eindices v)"
+  show ?thesis
+    unfolding iterate_neighbourhood_def CSR_assn_raw_def 
+    apply(rule ht_bind[where R = "\<lambda> r. ?big_assn * \<up> (r = sindices v)"])
+    subgoal
+      using lookup_rule by sep_auto
+    subgoal for vstarto
+     apply(clarsimp split!: option.split)
+      subgoal 
+        by sep_auto
+      subgoal 
+        apply sep_auto 
+        by (metis domIff domI)
+      subgoal
+        apply sep_auto
+        by (metis domI domIff)
+      subgoal for vstart vs
+        apply(rule ht_bind[where R = 
+             "\<lambda> r. ?big_assn * \<up> (Some vstart = sindices v) * \<up> (r = eindices v)"])
+        subgoal
+          using lookup_rule by sep_auto
+        subgoal for vendo
+          apply(cases vendo)
+           apply clarsimp
+          subgoal
+            apply sep_auto
+            by (metis domIff domI)
+          subgoal for vend
+            apply clarsimp
+            apply(rule ht_cons_prec[of _ "?help_assn vstart vend *
+                Gi \<mapsto>\<^sub>a nha * \<up> (vstart \<le> length nha \<and> vend < length nha) * F * acc_assn acc acci"
+                   "\<lambda> r. ?help_assn vstart vend 
+               * Gi \<mapsto>\<^sub>a nha * acc_assn (foldl (f v) acc (nths nha {vstart..vend})) r * F"])
+            subgoal
+              apply (sep_auto simp: domIff mod_pure_star_dist)
+              by (metis domI le_eq_less_or_eq option.sel)+
+            subgoal for res
+              apply (sep_auto  simp: domIff mod_pure_star_dist)
+               apply(rule forw_subst[of vs "nths nha {vstart..vend}"])
+              apply (metis option.sel domI)
+              by sep_auto 
+            subgoal
+              using iterate_range_rule[of acc_assn F "fi v" "f v" Gi nha vstart vend acc acci, OF assms]
+              by sep_auto
+            done
+          done
+        done
+      done
+    done
+qed
+
+lemma iterate_neighbourhood_rule:
+  assumes "\<And> acc acci x. <acc_assn acc acci * F> fi v x acci 
+            <\<lambda> r. acc_assn (f v acc x) r * F>"
+  shows "<CSR_assn nhlists Gi sindicesi eindicesi* acc_assn acc acci * F>
+         iterate_neighbourhood Gi sindicesi eindicesi v fi acci
+        <\<lambda> r. CSR_assn nhlists Gi sindicesi eindicesi* F* 
+              acc_assn (case nhlists v of None \<Rightarrow> acc
+                        | Some vs \<Rightarrow> foldl (f v) acc vs) r>"
+  using iterate_neighbourhood_raw_rule[of acc_assn F fi v f, OF assms, 
+      of nhlists Gi sindicesi eindicesi]
+  unfolding CSR_assn_def 
+  by sep_auto
+
+definition "weighted_CSR_assn_raw nhlists w Gi Wi sindicesi eindicesi nha ws sindices eindices= 
+  (Gi \<mapsto>\<^sub>a nha *  Wi \<mapsto>\<^sub>a ws * is_index_map sindices sindicesi
+      * is_index_map eindices eindicesi * 
+       \<up> (  dom eindices = dom sindices \<and> dom nhlists = dom sindices \<and>
+           (\<forall> v \<in> dom sindices. (the (sindices v) < length nha  \<and> the (eindices v) < length nha \<and>
+                   the (sindices v) < length ws  \<and> the (eindices v) < length ws) 
+                \<and> the (nhlists v) = nths nha {the (sindices v)..the (eindices v)} \<and> 
+                  (\<forall> u \<in> {the (sindices v)..the (eindices v)}. ws ! u = w v (nha ! u))) \<and>
+           (\<forall> u v. ({u, v} \<subseteq> dom sindices \<and> u \<noteq> v)
+              \<longrightarrow> {the (sindices v)..the (eindices v)} \<inter> {the (sindices u)..the (eindices v)} = {})
+         ))"
+
+definition "weighted_CSR_assn nhlists w Gi Wi sindicesi eindicesi = 
+  (\<exists>\<^sub>A nha ws sindices eindices. 
+      weighted_CSR_assn_raw nhlists w Gi Wi sindicesi eindicesi nha ws sindices eindices)"
+
+definition "weighted_CSR_assn_raw_alt nhlists w Gi Wi sindicesi eindicesi nha ws sindices eindices= 
+  (Gi \<mapsto>\<^sub>a nha *  Wi \<mapsto>\<^sub>a ws * is_index_map sindices sindicesi
+      * is_index_map eindices eindicesi * 
+       \<up> (  dom eindices = dom sindices \<and> dom nhlists = dom sindices \<and>
+           (\<forall> v \<in> dom sindices. (the (sindices v) < length nha  \<and> the (eindices v) < length nha \<and>
+                   the (sindices v) < length ws  \<and> the (eindices v) < length ws) 
+                \<and> the (nhlists v) = nths nha {the (sindices v)..the (eindices v)} \<and> 
+                  (\<forall> u \<in> {the (sindices v)..the (eindices v)}. 
+                          ws ! u = w v (the (nhlists v) ! (u - the (sindices v))))) \<and>
+           (\<forall> u v. ({u, v} \<subseteq> dom sindices \<and> u \<noteq> v)
+              \<longrightarrow> {the (sindices v)..the (eindices v)} \<inter> {the (sindices u)..the (eindices v)} = {})
+         ))"
+
+lemma weighted_CSR_assn_raw_alt_same: "weighted_CSR_assn_raw_alt = weighted_CSR_assn_raw"
+proof((rule ext)+, goal_cases)
+  case (1 nhlists w Gi Wi sindicesi eindicesi nha ws sindices eindices)
+  thus ?case
+    unfolding weighted_CSR_assn_raw_alt_def weighted_CSR_assn_raw_def
+    apply(rule ent_iffI)
+    apply(all \<open>sep_auto simp: domIff mod_pure_star_dist,
+             subst nth_shifted_by_lower_bound_of_nths_intervall\<close>)
+    by auto
+qed
+
+partial_function (heap) iterate_range_infoed where
+  "iterate_range_infoed arr info_arr start end fi acc=
+    (if start \<le> end then
+      do{ current \<leftarrow> Array.nth arr start;
+          current_info \<leftarrow> Array.nth info_arr start;
+          acc' \<leftarrow> fi current current_info acc;
+          iterate_range_infoed arr info_arr (Suc start) end fi acc'}
+     else return acc)"
+
+lemma iterate_range_infoed_rule:
+  assumes "\<And> acc acci x y. <acc_assn acc acci * F> fi x y acci 
+            <\<lambda> r. acc_assn (f acc (x, y)) r * F>"
+  shows "<arr \<mapsto>\<^sub>a list * info_arr \<mapsto>\<^sub>a info_list *
+          \<up> (start \<le> length list \<and> end < length list \<and>
+             start \<le> length info_list \<and> end < length info_list) *F * acc_assn acc acci>
+          iterate_range_infoed arr info_arr start end fi acci 
+       <\<lambda> r. arr \<mapsto>\<^sub>a list *  info_arr \<mapsto>\<^sub>a info_list * 
+        acc_assn (foldl f acc (zip (nths list {start..end}) (nths info_list {start..end}))) r * F>"
+proof(induction arbitrary: start acc acci rule: iterate_range_infoed.fixp_induct, goal_cases)
+  case 1
+  then show ?case
+    by simp
+next
+  case 2
+  then show ?case 
+    by simp
+next
+  case (3 fi start acc acci)
+  note IH = this
+  show ?case 
+     using assms(1) IH(1)[of "Suc start" "f acc _"]
+     by (sep_auto simp: nths_intervall_split_off_first[of start] split: if_split)
+ qed
+
+definition "iterate_weighted_neighbourhood Gi Wi sindicesi eindicesi v fi acci= 
+   do{ vstarto \<leftarrow> index_lookup v sindicesi;
+       case vstarto of None \<Rightarrow> return acci
+       | Some vstart \<Rightarrow> do{
+          vendo \<leftarrow> index_lookup v eindicesi;
+          let vend = the vendo;
+          iterate_range_infoed Gi Wi vstart vend (fi v) acci}}"
+
+lemma iterate_weighted_neighbourhood_raw_rule:
+  assumes "\<And> acc acci x y. <acc_assn acc acci * F> fi v x y acci 
+            <\<lambda> r. acc_assn (f v x y acc) r * F>"
+  shows "<weighted_CSR_assn_raw nhlists w Gi Wi sindicesi eindicesi nha ws sindices eindices
+        * acc_assn acc acci * F>
+         iterate_weighted_neighbourhood Gi Wi sindicesi eindicesi v fi acci
+      <\<lambda> r. weighted_CSR_assn_raw nhlists w Gi Wi sindicesi eindicesi nha ws sindices eindices* F* 
+              acc_assn (case nhlists v of None \<Rightarrow> acc
+                        | Some vs \<Rightarrow> foldl (\<lambda> acc x. f v x (w v x) acc) acc vs) r>"
+proof-
+  let ?big_assn = "Gi \<mapsto>\<^sub>a nha * Wi \<mapsto>\<^sub>a ws * is_index_map sindices sindicesi * is_index_map eindices eindicesi *
+     \<up> (dom eindices = dom sindices \<and>
+        dom nhlists = dom sindices \<and>
+        (\<forall>v\<in>dom sindices.
+            (the (sindices v) < length nha \<and>
+             the (eindices v) < length nha \<and>
+             the (sindices v) < length ws \<and> the (eindices v) < length ws) \<and>
+            the (nhlists v) = nths nha {the (sindices v)..the (eindices v)} \<and>
+            (\<forall>u\<in>{the (sindices v)..the (eindices v)}. ws ! u = w v (nha ! u))) \<and>
+        (\<forall>u v. {u, v} \<subseteq> dom sindices \<and> u \<noteq> v \<longrightarrow>
+               {the (sindices v)..the (eindices v)} \<inter> {the (sindices u)..the (eindices v)} = {})) *
+     acc_assn acc acci *
+     F"
+  let ?help_assn ="\<lambda> vstart vend. is_index_map sindices sindicesi * is_index_map eindices eindicesi *
+      \<up> (dom eindices = dom sindices \<and>
+        dom nhlists = dom sindices \<and>
+        (\<forall>v\<in>dom sindices.
+            the (sindices v) < length nha \<and>
+            the (eindices v) < length nha \<and>
+            the (sindices v) < length ws \<and>
+            the (eindices v) < length ws \<and>
+            the (nhlists v) = nths nha {the (sindices v)..the (eindices v)} \<and>
+            (\<forall>u\<in>{the (sindices v)..the (eindices v)}. ws ! u = w v (nha ! u))) \<and>
+        (\<forall>u v. u \<in> dom sindices \<and> v \<in> dom sindices \<and> u \<noteq> v \<longrightarrow>
+               the (sindices v) \<le> the (eindices v) \<longrightarrow> \<not> the (sindices u) \<le> the (eindices v))
+       \<and> vstart \<le> length nha \<and> vend < length nha \<and>  vstart \<le> length ws \<and> vend < length ws 
+       \<and> Some vstart = sindices v \<and> Some vend = eindices v)"
+  have assn_change:
+    "<acc_assn acc acci * F> fi v x y acci
+        <\<lambda>r. acc_assn (case (x, y) of (x, y) \<Rightarrow> f v x y acc) r * F>" for acc acci x y
+   using assms[of acc acci x y] by simp
+  show ?thesis
+    unfolding iterate_weighted_neighbourhood_def weighted_CSR_assn_raw_def 
+    apply(rule ht_bind[where R = "\<lambda> r. ?big_assn * \<up> (r = sindices v)"])
+    subgoal
+      using lookup_rule by sep_auto
+    subgoal for vstarto
+     apply(clarsimp split!: option.split)
+      subgoal 
+        by sep_auto
+      subgoal 
+        apply sep_auto 
+        by (metis domIff domI)
+      subgoal
+        apply sep_auto
+        by (metis domI domIff)
+      subgoal for vstart vs
+        apply(rule ht_bind[where R = 
+             "\<lambda> r. ?big_assn * \<up> (Some vstart = sindices v) * \<up> (r = eindices v)"])
+        subgoal
+          using lookup_rule by sep_auto
+        subgoal for vendo
+          apply(cases vendo)
+           apply clarsimp
+          subgoal
+            apply sep_auto
+            by (metis domIff domI)
+          subgoal for vend
+            apply clarsimp
+            apply(rule ht_cons_prec[of _ "?help_assn vstart vend *
+                Gi \<mapsto>\<^sub>a nha * Wi \<mapsto>\<^sub>a ws  * F * acc_assn acc acci"
+                   "\<lambda> r. ?help_assn vstart vend 
+               * Gi \<mapsto>\<^sub>a nha *  Wi \<mapsto>\<^sub>a ws * acc_assn (foldl (\<lambda> acc (x, y). f v x y acc) acc 
+                    (zip (nths nha {vstart..vend}) (nths ws {vstart..vend}))) r * F"])
+            subgoal
+              apply (sep_auto simp: domIff mod_pure_star_dist)
+              by (metis domI le_eq_less_or_eq option.sel)+
+            subgoal for res
+              apply (sep_auto  simp: domIff mod_pure_star_dist)
+              apply(rule forw_subst[of vs "nths nha {vstart..vend}"])
+              subgoal
+                apply(elim ballE[where x = v])
+                 apply (auto intro!: arg_cong[where f = "nths nha"])
+                by (metis option.sel)+
+              apply(subst zip_foldl_map[where y = "w v"])
+              subgoal
+                apply(rule nth_equalityI)
+                subgoal
+                  apply simp
+                  apply (subst length_nths_of_intervall)
+                   apply (metis option.sel domI)
+                  apply (subst length_nths_of_intervall)
+                   apply (metis option.sel domI)
+                  by simp
+                subgoal for i
+                  apply(subst (asm) length_nths_of_intervall)
+                     apply (metis option.sel domI)
+                  apply simp
+                  apply(subst nth_map)
+                  subgoal
+                     apply(subst length_nths_of_intervall)
+                     apply (metis option.sel domI)
+                     by simp
+                  apply(subst nth_of_nths_intervall_shifted_by_lower_bound)
+                  subgoal
+                    by (metis option.sel domI)
+                  subgoal
+                    by simp
+                  apply(subst nth_of_nths_intervall_shifted_by_lower_bound)
+                  subgoal
+                    by (metis option.sel domI)
+                  subgoal
+                    by simp
+                  apply(elim ballE[of _ _ v])
+                  subgoal
+                    apply auto
+                    apply(elim ballE[of _ _ "i + vstart"])
+                    subgoal
+                      by auto
+                    subgoal
+                      unfolding eq_commute[of "Some vend"]  eq_commute[of "Some vstart"]
+                      by simp
+                    done
+                  by auto
+                done
+              by sep_auto
+            subgoal
+              using iterate_range_infoed_rule[of acc_assn F "fi v" "\<lambda>acc (x, y). f v x y acc",
+                     OF assn_change, of Gi nha Wi ws vstart vend acc acci]
+              by sep_auto
+            done
+          done
+        done
+      done
+    done
+qed
+
+lemma iterate_weighted_neighbourhood_rule:
+  assumes "\<And> acc acci x y. <acc_assn acc acci * F> fi v x y acci 
+            <\<lambda> r. acc_assn (f v x y acc) r * F>"
+  shows "<weighted_CSR_assn nhlists w Gi Wi sindicesi eindicesi * acc_assn acc acci * F>
+         iterate_weighted_neighbourhood Gi Wi sindicesi eindicesi v fi acci
+       <\<lambda> r. weighted_CSR_assn nhlists w Gi Wi sindicesi eindicesi* F* 
+             acc_assn (case nhlists v of None \<Rightarrow> acc
+                        | Some vs \<Rightarrow> foldl (\<lambda> acc x. f v x (w v x) acc) acc vs) r>"
+  unfolding weighted_CSR_assn_def ex_assn_move_out(1)
+proof((rule ht_ex_pre_and_post_I)+, goal_cases)
+  case (1 nha ws sindices eindices)
+  thus ?case
+  using iterate_weighted_neighbourhood_raw_rule[of acc_assn F fi v f, OF assms, 
+      of nhlists w Gi Wi sindicesi eindicesi nha ws sindices eindices acc acci]
+  by simp
+qed
+end
+
+locale CSR_array 
+begin
+
+definition "CSR_assn_raw nhlists Gi sindicesi eindicesi nha sindices eindices= 
+  (Gi \<mapsto>\<^sub>a nha * sindicesi \<mapsto>\<^sub>a sindices
+      * eindicesi \<mapsto>\<^sub>a eindices* 
+       \<up> (
+          dom nhlists \<subseteq> {0..<length sindices} \<and> dom nhlists \<subseteq> {0..<length eindices} \<and>
+          length sindices = length eindices \<and>
+          (\<forall> v \<in> dom nhlists. sindices ! v < length nha  \<and> eindices ! v < length nha
+               \<and> the (nhlists v) = nths nha {sindices ! v..eindices ! v} \<and>
+           the (nhlists v) = nths nha {sindices ! v..eindices ! v}) \<and>
+          (\<forall> v. v \<notin> dom nhlists \<and> v < length sindices \<longrightarrow>
+               sindices ! v > eindices ! v)
+         \<and> (\<forall> u v. ({u, v} \<subseteq> dom nhlists \<and> u \<noteq> v)
+             \<longrightarrow> {sindices ! v..eindices ! v} \<inter> {sindices ! u..eindices ! v} = {})
+        )
+   )"
+
+definition "CSR_assn nhlists Gi sindicesi eindicesi = 
+  (\<exists>\<^sub>A nha sindices eindices. CSR_assn_raw nhlists Gi sindicesi eindicesi nha sindices eindices)"
+
+definition "iterate_neighbourhood Gi sindicesi eindicesi v fi acci= 
+   do{ n \<leftarrow> Array.len sindicesi;
+      if v \<ge> n then return acci
+      else do{
+        vstart \<leftarrow> Array.nth sindicesi v;
+        vend \<leftarrow> Array.nth eindicesi v;
+          iterate_range Gi vstart vend (fi v) acci}}"
+
+lemma iterate_neighbourhood_raw_rule:
+  assumes "\<And> acc acci x. <acc_assn acc acci * F> fi v x acci 
+            <\<lambda> r. acc_assn (f v acc x) r * F>"
+  shows "<CSR_assn_raw nhlists Gi sindicesi eindicesi nha sindices eindices* acc_assn acc acci * F>
+         iterate_neighbourhood Gi sindicesi eindicesi v fi acci
+        <\<lambda> r. CSR_assn_raw nhlists Gi sindicesi eindicesi nha sindices eindices* F* 
+              acc_assn (foldl (f v) acc (case nhlists v of None \<Rightarrow> Nil | Some vs \<Rightarrow> vs)) r>"
+proof-
+  let ?big_assn = "Gi \<mapsto>\<^sub>a nha * sindicesi \<mapsto>\<^sub>a sindices * eindicesi \<mapsto>\<^sub>a eindices *
+     \<up> (dom nhlists \<subseteq> {0..<length sindices} \<and>
+        dom nhlists \<subseteq> {0..<length eindices} \<and>
+        length sindices = length eindices \<and>
+        (\<forall>v\<in>dom nhlists.
+            sindices ! v < length nha \<and>
+            eindices ! v < length nha \<and>
+            the (nhlists v) = nths nha {sindices ! v..eindices ! v} \<and>
+            the (nhlists v) = nths nha {sindices ! v..eindices ! v}) \<and>
+        (\<forall>v. v \<notin> dom nhlists \<and> v < length sindices \<longrightarrow> eindices ! v < sindices ! v) \<and>
+        (\<forall>u v. {u, v} \<subseteq> dom nhlists \<and> u \<noteq> v \<longrightarrow>
+               {sindices ! v..eindices ! v} \<inter> {sindices ! u..eindices ! v} = {})) *
+     acc_assn acc acci *
+     F"
+  let ?help_assn ="\<lambda> vstart vend n. sindicesi \<mapsto>\<^sub>a sindices * eindicesi \<mapsto>\<^sub>a eindices *
+     \<up> (dom nhlists \<subseteq> {0..<length sindices} \<and>
+        dom nhlists \<subseteq> {0..<length eindices} \<and>
+        length sindices = length eindices \<and>
+        (\<forall>v\<in>dom nhlists.
+            sindices ! v < length nha \<and>
+            eindices ! v < length nha \<and> the (nhlists v) = nths nha {sindices ! v..eindices ! v}) \<and>
+        (\<forall>v. v \<notin> dom nhlists \<and> v < length sindices \<longrightarrow> eindices ! v < sindices ! v) \<and>
+        (\<forall>u v. u \<in> dom nhlists \<and> v \<in> dom nhlists \<and> u \<noteq> v \<longrightarrow>
+               sindices ! v \<le> eindices ! v \<longrightarrow> \<not> sindices ! u \<le> eindices ! v)) *
+        \<up> (vstart \<le> length nha \<and> vend < length nha \<and>
+                           n = length sindices \<and> vstart = sindices ! v \<and> vend = eindices ! v)"
+  show ?thesis
+    unfolding iterate_neighbourhood_def CSR_assn_raw_def 
+    apply(rule ht_bind[where R = "\<lambda> r. ?big_assn * \<up> (r = length sindices)"])
+    subgoal
+       by sep_auto
+    apply(clarsimp split!: if_split option.split)
+    subgoal for n
+      by sep_auto
+    subgoal for n vs
+      by sep_auto
+    subgoal for n
+      by (sep_auto elim:  allE[of "\<lambda> v. v \<notin> dom nhlists \<and> v < length eindices 
+                   \<longrightarrow> eindices ! v < sindices ! v" v] simp: iterate_range.simps)
+    subgoal for n vs
+        apply(rule ht_bind[where R = 
+             "\<lambda> r. ?big_assn * \<up> (n = length sindices \<and> r = sindices ! v)"])
+      subgoal
+        by sep_auto
+      subgoal for vstart
+        apply(rule ht_bind[where R = 
+             "\<lambda> r. ?big_assn * \<up> (n = length sindices \<and> vstart = sindices ! v \<and> r = eindices ! v)"])
+        subgoal
+           by sep_auto
+          subgoal for vend
+            apply clarsimp
+            apply(rule ht_cons_prec[of _ "?help_assn vstart vend n *  Gi \<mapsto>\<^sub>a nha * F * acc_assn acc acci"
+                   "\<lambda> r. ?help_assn vstart vend  n * Gi \<mapsto>\<^sub>a nha * 
+                       acc_assn (foldl (f v) acc (nths nha {vstart..vend})) r * F"])
+            subgoal
+              apply (sep_auto simp: domIff mod_pure_star_dist)
+              by (metis domI le_eq_less_or_eq option.sel)+
+            subgoal for res
+              apply (sep_auto simp: domIff mod_pure_star_dist)
+               apply(rule forw_subst[of vs "nths nha {vstart..vend}"])
+              apply (metis domI option.sel)
+              by sep_auto 
+            subgoal
+              using iterate_range_rule[of acc_assn F "fi v" "f v" Gi nha vstart vend acc acci, OF assms]
+              by sep_auto
+            done
+          done
+        done
+      done
+qed
+
+lemma iterate_neighbourhood_rule:
+  assumes "\<And> acc acci x. <acc_assn acc acci * F> fi v x acci 
+            <\<lambda> r. acc_assn (f v acc x) r * F>"
+  shows "<CSR_assn nhlists Gi sindicesi eindicesi* acc_assn acc acci * F>
+         iterate_neighbourhood Gi sindicesi eindicesi v fi acci
+        <\<lambda> r. CSR_assn nhlists Gi sindicesi eindicesi* F* 
+              acc_assn (foldl (f v) acc (case nhlists v of None \<Rightarrow> Nil | Some vs \<Rightarrow> vs)) r>"
+  using iterate_neighbourhood_raw_rule[of acc_assn F fi v f, OF assms, 
+      of nhlists Gi sindicesi eindicesi]
+  unfolding CSR_assn_def 
+  by sep_auto
+
+definition "weighted_CSR_assn_raw nhlists w Gi Wi sindicesi eindicesi nha ws sindices eindices= 
+  (Gi \<mapsto>\<^sub>a nha * sindicesi \<mapsto>\<^sub>a sindices * eindicesi \<mapsto>\<^sub>a eindices * Wi \<mapsto>\<^sub>a ws* 
+       \<up> (
+          dom nhlists \<subseteq> {0..<length sindices} \<and> dom nhlists \<subseteq> {0..<length eindices} \<and>
+          length sindices = length eindices \<and>
+          (\<forall> v \<in> dom nhlists. sindices ! v < length nha  \<and> eindices ! v < length nha
+               \<and> the (nhlists v) = nths nha {sindices ! v..eindices ! v} \<and>
+               sindices ! v < length ws  \<and> eindices ! v < length ws \<and>
+           the (nhlists v) = nths nha {sindices ! v..eindices ! v} \<and> 
+            (\<forall> u \<in> {(sindices ! v)..(eindices ! v)}. ws ! u = w v (nha ! u))) \<and>
+          (\<forall> v. v \<notin> dom nhlists \<and> v < length sindices \<longrightarrow>
+               sindices ! v > eindices ! v)
+         \<and> (\<forall> u v. ({u, v} \<subseteq> dom nhlists \<and> u \<noteq> v)
+             \<longrightarrow> {sindices ! v..eindices ! v} \<inter> {sindices ! u..eindices ! v} = {})
+        )
+      )"
+
+definition "weighted_CSR_assn nhlists w Gi Wi sindicesi eindicesi = 
+  (\<exists>\<^sub>A nha ws sindices eindices. 
+      weighted_CSR_assn_raw nhlists w Gi Wi sindicesi eindicesi nha ws sindices eindices)"
+
+definition "weighted_CSR_assn_raw_alt nhlists w Gi Wi sindicesi eindicesi nha ws sindices eindices= 
+  (Gi \<mapsto>\<^sub>a nha * sindicesi \<mapsto>\<^sub>a sindices * eindicesi \<mapsto>\<^sub>a eindices * Wi \<mapsto>\<^sub>a ws* 
+       \<up> (
+          dom nhlists \<subseteq> {0..<length sindices} \<and> dom nhlists \<subseteq> {0..<length eindices} \<and>
+          length sindices = length eindices \<and>
+          (\<forall> v \<in> dom nhlists. sindices ! v < length nha  \<and> eindices ! v < length nha
+               \<and> the (nhlists v) = nths nha {sindices ! v..eindices ! v} \<and>
+               sindices ! v < length ws  \<and> eindices ! v < length ws \<and>
+           the (nhlists v) = nths nha {sindices ! v..eindices ! v} \<and> 
+            (\<forall> u \<in> {(sindices ! v)..(eindices ! v)}. ws ! u = w v (the (nhlists v) ! (u - sindices ! v)))) \<and>
+          (\<forall> v. v \<notin> dom nhlists \<and> v < length sindices \<longrightarrow>
+               sindices ! v > eindices ! v)
+         \<and> (\<forall> u v. ({u, v} \<subseteq> dom nhlists \<and> u \<noteq> v)
+             \<longrightarrow> {sindices ! v..eindices ! v} \<inter> {sindices ! u..eindices ! v} = {})
+        )
+      )"
+
+lemma weighted_CSR_assn_raw_alt_same: "weighted_CSR_assn_raw_alt = weighted_CSR_assn_raw"
+proof((rule ext)+, goal_cases)
+  case (1 nhlists w Gi Wi sindicesi eindicesi nha ws sindices eindices)
+  thus ?case
+    unfolding weighted_CSR_assn_raw_alt_def weighted_CSR_assn_raw_def
+    apply(rule ent_iffI)
+    apply(all \<open>sep_auto simp: domIff mod_pure_star_dist,
+             subst nth_shifted_by_lower_bound_of_nths_intervall\<close>)
+    by auto
+qed
+
+definition "iterate_weighted_neighbourhood Gi Wi sindicesi eindicesi v fi acci= 
+   do{n \<leftarrow> Array.len sindicesi;
+      if v \<ge> n then return acci
+      else do{
+        vstart \<leftarrow> Array.nth sindicesi v;
+        vend \<leftarrow> Array.nth eindicesi v;
+        iterate_range_infoed Gi Wi vstart vend (fi v) acci}}"
+
+lemma iterate_weighted_neighbourhood_raw_rule:
+  assumes "\<And> acc acci x y. <acc_assn acc acci * F> fi v x y acci 
+            <\<lambda> r. acc_assn (f v x y acc) r * F>"
+  shows "<weighted_CSR_assn_raw nhlists w Gi Wi sindicesi eindicesi nha ws sindices eindices
+        * acc_assn acc acci * F>
+         iterate_weighted_neighbourhood Gi Wi sindicesi eindicesi v fi acci
+      <\<lambda> r. weighted_CSR_assn_raw nhlists w Gi Wi sindicesi eindicesi nha ws sindices eindices* F* 
+              acc_assn (case nhlists v of None \<Rightarrow> acc
+                        | Some vs \<Rightarrow> foldl (\<lambda> acc x. f v x (w v x) acc) acc vs) r>"
+proof-
+  let ?big_assn = "Gi \<mapsto>\<^sub>a nha * sindicesi \<mapsto>\<^sub>a sindices * eindicesi \<mapsto>\<^sub>a eindices * Wi \<mapsto>\<^sub>a ws *
+     \<up> (dom nhlists \<subseteq> {0..<length sindices} \<and>
+        dom nhlists \<subseteq> {0..<length eindices} \<and>
+        length sindices = length eindices \<and>
+        (\<forall>v\<in>dom nhlists.
+            sindices ! v < length nha \<and>
+            eindices ! v < length nha \<and>
+            the (nhlists v) = nths nha {sindices ! v..eindices ! v} \<and>
+            sindices ! v < length ws \<and>
+            eindices ! v < length ws \<and>
+            the (nhlists v) = nths nha {sindices ! v..eindices ! v} \<and>
+            (\<forall>u\<in>{sindices ! v..eindices ! v}. ws ! u = w v (nha ! u))) \<and>
+        (\<forall>v. v \<notin> dom nhlists \<and> v < length sindices \<longrightarrow> eindices ! v < sindices ! v) \<and>
+        (\<forall>u v. {u, v} \<subseteq> dom nhlists \<and> u \<noteq> v \<longrightarrow> {sindices ! v..eindices ! v} \<inter> {sindices ! u..eindices ! v} = {})) *
+     acc_assn acc acci *
+     F"
+  let ?help_assn ="\<lambda> vstart vend n vs.  sindicesi \<mapsto>\<^sub>a sindices * eindicesi \<mapsto>\<^sub>a eindices * 
+     \<up> (dom nhlists \<subseteq> {0..<length sindices} \<and>
+        dom nhlists \<subseteq> {0..<length eindices} \<and>
+        length sindices = length eindices \<and>
+        (\<forall>v\<in>dom nhlists.
+            sindices ! v < length nha \<and>
+            eindices ! v < length nha \<and>
+            the (nhlists v) = nths nha {sindices ! v..eindices ! v} \<and>
+            sindices ! v < length ws \<and>
+            eindices ! v < length ws \<and>
+            the (nhlists v) = nths nha {sindices ! v..eindices ! v} \<and>
+            (\<forall>u\<in>{sindices ! v..eindices ! v}. ws ! u = w v (nha ! u))) \<and>
+        (\<forall>v. v \<notin> dom nhlists \<and> v < length sindices \<longrightarrow> eindices ! v < sindices ! v) \<and>
+        (\<forall>u v. u \<in> dom nhlists \<and> v \<in> dom nhlists \<and> u \<noteq> v \<longrightarrow>
+               sindices ! v \<le> eindices ! v \<longrightarrow> \<not> sindices ! u \<le> eindices ! v) \<and>
+          n = length sindices \<and> vstart = sindices ! v \<and> vend = eindices ! v \<and>
+          vstart \<le> length nha \<and> vend < length nha \<and>
+                         vstart \<le> length ws \<and> vend < length ws \<and>
+           vs = nths nha {sindices ! v..eindices ! v})"
+  have assn_change:
+    "<acc_assn acc acci * F> fi v x y acci
+        <\<lambda>r. acc_assn (case (x, y) of (x, y) \<Rightarrow> f v x y acc) r * F>" for acc acci x y
+   using assms[of acc acci x y] by simp
+  show ?thesis
+    unfolding iterate_weighted_neighbourhood_def weighted_CSR_assn_raw_def 
+    apply(rule ht_bind[where R = "\<lambda> r. ?big_assn * \<up> (r = length sindices)"])
+    subgoal
+       by sep_auto
+    apply(clarsimp split!: if_split option.split)
+    subgoal for n
+      by sep_auto
+    subgoal for n vs
+      by sep_auto
+    subgoal for n
+      by (sep_auto elim:  allE[of "\<lambda> v. v \<notin> dom nhlists \<and> v < length eindices 
+                   \<longrightarrow> eindices ! v < sindices ! v" v] simp: iterate_range_infoed.simps)
+    subgoal for n vs
+        apply(rule ht_bind[where R = 
+             "\<lambda> r. ?big_assn * \<up> (n = length sindices \<and> r = sindices ! v)"])
+      subgoal
+        by sep_auto
+      subgoal for vstart
+        apply(rule ht_bind[where R = 
+             "\<lambda> r. ?big_assn * \<up> (n = length sindices \<and> vstart = sindices ! v \<and> r = eindices ! v)"])
+        subgoal
+           by sep_auto
+       subgoal for vend
+            apply clarsimp
+          apply(rule ht_cons_prec[of _ "?help_assn vstart vend n vs*  Gi \<mapsto>\<^sub>a nha * Wi \<mapsto>\<^sub>a ws* F * acc_assn acc acci"
+                   "\<lambda> r. ?help_assn vstart vend n vs* Gi \<mapsto>\<^sub>a nha * Wi \<mapsto>\<^sub>a ws* 
+                      acc_assn (foldl (\<lambda> acc (x, y). f v x y acc) acc 
+                    (zip (nths nha {vstart..vend}) (nths ws {vstart..vend}))) r * F"])
+            subgoal
+              apply (sep_auto simp: domIff mod_pure_star_dist)
+              by (metis domI le_eq_less_or_eq option.sel)+
+            subgoal for res
+              apply sep_auto
+              apply(rule forw_subst[of vs "nths nha {vstart..vend}"])
+               apply force
+              apply(subst zip_foldl_map[where y = "w v"])
+              subgoal
+                apply(rule nth_equalityI)
+                subgoal
+                  apply simp
+                  apply (subst length_nths_of_intervall)
+                   apply (metis option.sel domI)
+                  apply (subst length_nths_of_intervall)
+                   apply (metis option.sel domI)
+                  by simp
+                subgoal for i
+                  apply(subst (asm) length_nths_of_intervall)
+                     apply (metis option.sel domI)
+                  apply simp
+                  apply(subst nth_map)
+                  subgoal
+                     apply(subst length_nths_of_intervall)
+                     apply (metis option.sel domI)
+                     by simp
+                  apply(subst nth_of_nths_intervall_shifted_by_lower_bound)
+                  subgoal
+                    by (metis option.sel domI)
+                  subgoal
+                    by simp
+                  apply(subst nth_of_nths_intervall_shifted_by_lower_bound)
+                  subgoal
+                    by (metis option.sel domI)
+                  subgoal
+                    by simp
+                  by(auto elim: ballE[of _ _ v])
+                done
+              subgoal
+                by sep_auto
+              subgoal
+                by sep_auto
+              subgoal
+                by sep_auto
+              subgoal
+                by sep_auto
+              subgoal
+                by sep_auto
+              subgoal
+                by sep_auto
+              subgoal 
+                apply sep_auto
+                by (metis domI option.sel)
+              subgoal
+                by sep_auto
+              subgoal
+                by sep_auto
+              subgoal
+                apply sep_auto
+                by (metis domI option.sel)
+              subgoal 
+                apply sep_auto
+                by force
+              subgoal
+                by sep_auto
+              subgoal
+                apply sep_auto
+                by blast
+              done
+            subgoal
+              using iterate_range_infoed_rule[of acc_assn F "fi v" "\<lambda>acc (x, y). f v x y acc",
+                     OF assn_change, of Gi nha Wi ws vstart vend acc acci]
+              by sep_auto
+            done
+          done
+        done
+      done
+qed
+
+lemma iterate_weighted_neighbourhood_rule:
+  assumes "\<And> acc acci x y. <acc_assn acc acci * F> fi v x y acci 
+            <\<lambda> r. acc_assn (f v x y acc) r * F>"
+  shows "<weighted_CSR_assn nhlists w Gi Wi sindicesi eindicesi * acc_assn acc acci * F>
+         iterate_weighted_neighbourhood Gi Wi sindicesi eindicesi v fi acci
+       <\<lambda> r. weighted_CSR_assn nhlists w Gi Wi sindicesi eindicesi* F* 
+              acc_assn (case nhlists v of None \<Rightarrow> acc
+                        | Some vs \<Rightarrow> foldl (\<lambda> acc x. f v x (w v x) acc) acc vs) r>"
+  unfolding weighted_CSR_assn_def ex_assn_move_out(1)
+proof((rule ht_ex_pre_and_post_I)+, goal_cases)
+  case (1 nha ws sindices eindices)
+  thus ?case
+  using iterate_weighted_neighbourhood_raw_rule[of acc_assn F fi v f, OF assms, 
+      of nhlists w Gi Wi sindicesi eindicesi nha ws sindices eindices acc acci]
+  by simp
+qed
+end
+
+locale imp_map_copy = imp_map +
+  constrains is_map :: "('k \<rightharpoonup> 'v) \<Rightarrow> 'm \<Rightarrow> assn"
+  fixes copy :: "'m \<Rightarrow> 'm Heap"
+  assumes copy_rule[sep_heap_rules]: 
+    "<is_map m p> copy p <\<lambda>r. is_map m p * is_map m r>"
+
+definition "iam_copy m = 
+  do {l \<leftarrow> Array.len m;
+      m' \<leftarrow> Array.new l undefined;
+      blit m 0 m' 0 l;
+      return m'}"
+
+lemma iam_copy_rule:
+  "<is_iam m p> iam_copy p <\<lambda>r. is_iam m p * is_iam m r>"
+  unfolding is_iam_def iam_copy_def
+  by sep_auto
+
+interpretation iam_copy: imp_map_copy is_iam iam_copy
+  using iam_copy_rule
+  by unfold_locales
+
+
+(*
+definition "stack_assn = (\<lambda> stack (stackarr, sp) . 
+              (\<exists>\<^sub>A xs. stackarr \<mapsto>\<^sub>a xs * \<up> (sp < length xs \<and> take sp xs =  rev stack)))"
+
+definition "push_to_stack stack x = "
+
+  oops
+definition "stack_assn_raw stack stacktail stackarr sp = stackarr \<mapsto>"
+*)
+
