Set_Graphs/Graph_Algorithms/Dist_BFS.thy
@@ -1,0 +1,11 @@
+theory Dist_BFS
+  imports BFS_2
+begin
+
+locale Dist_BFS = 
+BFS where expand_tree = expand_tree for
+expand_tree::"'adjmap \<Rightarrow> 'vset \<Rightarrow> 'vset \<Rightarrow> 'adjmap" +
+fixes next_frontier_and_visited
+
+
+
